src/compiler/meta/OCL_compiler_meta_UML.thy
@@ -78,7 +78,8 @@ datatype ocl_ty =           OclTy_base_void
                           | OclTy_class_pre string (* class name, untyped *) (* FIXME perform the typing separately *)
                           | OclTy_class ocl_ty_class  (* class name, typed *)
                           | OclTy_collection ocl_collection ocl_ty
-                          | OclTy_raw string (* denoting raw HOL-type *)
+                          | OclTy_pair ocl_ty ocl_ty
+                          | OclTy_raw string (* denoting raw HOL-type *) (* FIXME to be removed *)
 
 
 datatype ocl_association_type = OclAssTy_native_attribute
@@ -128,7 +129,8 @@ definition "T_lambdas = List.fold T_lambda"
 subsection{* Class Translation Preliminaries *}
 
 definition "const_oid = ''oid''"
-definition "const_oid_list = ''list''"
+definition "var_ty_list = ''list''"
+definition "var_ty_prod = ''prod''"
 definition "const_oclany = ''OclAny''"
 
 definition "single_multip = (\<lambda> OclMult l _ \<Rightarrow>
@@ -310,12 +312,14 @@ fun_quick str_hol_of_ty where
    |"str_hol_of_ty OclTy_base_unlimitednatural = ''nat''"
    |"str_hol_of_ty OclTy_base_real = ''real''"
    |"str_hol_of_ty OclTy_base_string = ''string''"
-   |"str_hol_of_ty (OclTy_class ty_obj) = flatten [TyObj_name ty_obj, '' '', const_oid_list]"
+   |"str_hol_of_ty (OclTy_class ty_obj) = flatten [TyObj_name ty_obj, '' '', var_ty_list]"
    |"str_hol_of_ty (OclTy_raw s) = s"
 
 fun_quick str_hol_of_ty_all where
-    "str_hol_of_ty_all f b (OclTy_collection _ ty_obj) = 
-       f (b const_oid_list) [str_hol_of_ty_all f b ty_obj]"
+    "str_hol_of_ty_all f b (OclTy_collection _ ty) = 
+       f (b var_ty_list) [str_hol_of_ty_all f b ty]"
+   |"str_hol_of_ty_all f b (OclTy_pair ty1 ty2) = 
+       f (b var_ty_prod) [str_hol_of_ty_all f b ty1, str_hol_of_ty_all f b ty2]"
    |"str_hol_of_ty_all f b (OclTy_class_pre _) = b const_oid"
    |"str_hol_of_ty_all f b s = b (str_hol_of_ty s)"
 
